MinimunLogic/Complete/Lindenbaum_Kripke.v
@@ -4,7 +4,6 @@ Require Import Coq.Logic.Classical_Pred_Type.
 Require Import Logic.lib.Bijection.
 Require Import Logic.lib.Countable.
 Require Import Logic.GeneralLogic.Base.
-Require Import Logic.GeneralLogic.HenkinCompleteness.
 Require Import Logic.GeneralLogic.KripkeModel.
 Require Import Logic.MinimunLogic.Complete.ContextProperty_Kripke.
 
@@ -16,95 +15,12 @@ Import KripkeModelNotation_Intuitionistic.
 Section Lindenbaum_Kripke.
 
 Context {L: Language}
-        {nL: NormalLanguage L}
-        {pL: PropositionalLanguage L}
-        {Gamma: ProofTheory L}
-        {nGamma: NormalProofTheory L Gamma}
-        {mpGamma: MinimunPropositionalLogic L Gamma}
-        {ipGamma: IntuitionisticPropositionalLogic L Gamma}.
+        {Gamma: ProofTheory L}.
 
 Hypothesis CE: Countable expr.
 
-Lemma Lindenbaum_lemma:
-  forall Phi x,
-    ~ Phi |-- x ->
-    exists Psi,
-      Included _ Phi Psi /\
-      ~ Psi |-- x /\
-      derivable_closed Psi /\
-      orp_witnessed Psi /\
-      consistent Psi.
-Proof.
-  intros.
-  set (step :=
-          fun n Phi x0 =>
-             Phi x0 \/
-            (CE x0 n /\
-             ~ (Union _ Phi (Singleton _ x0)) |-- x)).
-  exists (LindenbaumConstruction step Phi).
-  assert (Included expr Phi (LindenbaumConstruction step Phi) /\
-          ~ LindenbaumConstruction step Phi |-- x /\
-          (~ LindenbaumConstruction step Phi |-- x ->
-           derivable_closed (LindenbaumConstruction step Phi)) /\
-          (~ LindenbaumConstruction step Phi |-- x ->
-           orp_witnessed (LindenbaumConstruction step Phi))).
-  Focus 2. {
-    destruct H0 as [? [? [? ?]]].
-    split; [| split; [| split; [| split]]]; auto.
-    rewrite consistent_spec.
-    intro; apply H1.
-    pose proof deduction_falsep_elim _ x H4.
-    auto.
-  } Unfocus.
-  split; [| split; [| split]].
-  + apply (Lindenbaum_spec_included _ _ 0).
-  + apply (Lindenbaum_spec_pos _ _
-            (fun xs => |-- multi_imp xs x)
-            (fun Phi => Phi |-- x)).
-    - intros; apply derivable_provable.
-    - intros ? ? ? ?; left; auto.
-    - apply H.
-    - intros.
-      destruct (Classical_Prop.classic (exists x0, CE x0 n /\ ~ (Union _ S (Singleton _ x0)) |-- x)) as [[x0 [? ?]] |].
-      * intro; apply H2; clear H2.
-        eapply deduction_weaken; [| exact H3].
-        hnf; intros ? [? | [? ?]]; [left; auto |].
-        pose proof in_inj _ _ CE _ _ _ H1 H2.
-        subst; right; constructor.
-      * intro; apply H0; clear H0.
-        eapply deduction_weaken; [| exact H2].
-        hnf; intros ? [? | [? ?]]; [auto |].
-        exfalso; apply H1; clear H1.
-        exists x0; auto.
-  + intros; hnf; intros.
-    destruct (im_inj _ _ CE x0) as [n ?].
-    apply (Lindenbaum_spec_neg _ _ _ (S n)).
-    simpl.
-    unfold step at 1.
-    right; split; auto.
-    intro.
-    rewrite deduction_theorem in H3.
-    eapply deduction_weaken in H3; [| apply (Lindenbaum_spec_included _ _ n)].
-    pose proof deduction_modus_ponens _ _ _ H1 H3.
-    auto.
-  + intros; hnf; intros x0 y0 ?.
-    destruct (im_inj _ _ CE x0) as [nx ?].
-    destruct (im_inj _ _ CE y0) as [ny ?].
-    assert (LindenbaumChain step Phi (S nx) x0 \/ LindenbaumChain step Phi (S ny) y0) as HH;
-      [| destruct HH as [HH | HH]; apply Lindenbaum_spec_neg in HH; auto].
-    simpl.
-    unfold step at 1 3.
-    assert (~ Union _ (LindenbaumChain step Phi nx) (Singleton _ x0) |-- x \/
-            ~ Union _ (LindenbaumChain step Phi ny) (Singleton _ y0) |-- x) as HH;
-      [| destruct HH as [HH | HH]; auto].
-    apply Classical_Prop.not_and_or; intros [? ?].
-    rewrite deduction_theorem in H4, H5.
-    eapply deduction_weaken in H4; [| apply (Lindenbaum_spec_included _ _ nx)].
-    eapply deduction_weaken in H5; [| apply (Lindenbaum_spec_included _ _ ny)].
-    pose proof deduction_orp_elim (LindenbaumConstruction step Phi) x0 y0 x H4 H5.
-    apply (derivable_assum _ (x0 || y0)) in H1.
-    pose proof deduction_modus_ponens _ _ _ H1 H6.
-    auto.
-Qed.
+Lemma Lindenbaum_constructable_DS: forall P,
+  
+    Lindenbaum_constructable P derivable_closed.
 
 End Lindenbaum_Kripke.
