MinimunLogic/DeepEmbedded/Complete_Kripke.v
@@ -1,0 +1,214 @@
+Require Import Coq.Logic.Classical_Prop.
+Require Import Logic.lib.Ensembles_ext.
+Require Import Logic.lib.Bijection.
+Require Import Logic.lib.Countable.
+Require Import Logic.GeneralLogic.Base.
+Require Import Logic.GeneralLogic.ProofTheory.BasicSequentCalculus.
+Require Import Logic.GeneralLogic.KripkeModel.
+Require Import Logic.GeneralLogic.Semantics.Kripke.
+Require Import Logic.GeneralLogic.Complete.ContextProperty.
+Require Import Logic.GeneralLogic.Complete.ContextProperty_Kripke.
+Require Import Logic.GeneralLogic.Complete.Lindenbaum.
+Require Import Logic.GeneralLogic.Complete.Canonical_Kripke.
+Require Import Logic.MinimunLogic.Syntax.
+Require Import Logic.MinimunLogic.ProofTheory.Minimun2.
+Require Import Logic.MinimunLogic.Semantics.Kripke.
+Require Import Logic.MinimunLogic.Complete.ContextProperty_Kripke.
+Require Import Logic.MinimunLogic.Complete.Truth_Kripke.
+Require Import Logic.PropositionalLogic.Complete.Complete_Kripke.
+Require Logic.PropositionalLogic.DeepEmbedded.PropositionalLanguage.
+Require Logic.PropositionalLogic.DeepEmbedded.IntuitionisticLogic.
+Require Logic.PropositionalLogic.DeepEmbedded.DeMorganLogic.
+Require Logic.PropositionalLogic.DeepEmbedded.GodelDummettLogic.
+Require Logic.PropositionalLogic.DeepEmbedded.ClassicalLogic.
+Require Logic.PropositionalLogic.DeepEmbedded.KripkeSemantics.
+
+Local Open Scope logic_base.
+Local Open Scope syntax.
+Local Open Scope kripke_model.
+Local Open Scope kripke_model_class.
+Import PropositionalLanguageNotation.
+Import KripkeModelFamilyNotation.
+Import KripkeModelNotation_Intuitionistic.
+Import KripkeModelClass.
+
+Section Complete.
+
+Context (Var: Type) (CV: Countable Var).
+
+Instance L: Language := PropositionalLanguage.L Var.
+Instance nL: NormalLanguage L := PropositionalLanguage.nL Var.
+Instance pL: PropositionalLanguage L := PropositionalLanguage.pL Var.
+
+Instance Intuitionistic_G: ProofTheory L := IntuitionisticLogic.G Var.
+Instance DeMorgan_G: ProofTheory L := DeMorganLogic.G Var.
+Instance GodelDummett_G: ProofTheory L := GodelDummettLogic.G Var.
+Instance Classical_G: ProofTheory L := ClassicalLogic.G Var.
+Instance Kripke_MD: Model := KripkeSemantics.MD Var.
+Instance Kripke_kMD: KripkeModel Kripke_MD := KripkeSemantics.kMD Var.
+Instance Kripke_R (M: Kmodel): Relation (Kworlds M) := KripkeSemantics.R Var M.
+Instance Kripke_SM: Semantics L Kripke_MD := KripkeSemantics.SM Var.
+Instance Kripke_kpSM (M: Kmodel): KripkePropositionalSemantics L Kripke_MD M Kripke_SM := KripkeSemantics.kpSM Var M.
+
+Section General_Completeness.
+
+Context {Gamma: ProofTheory L}
+        {nGamma: NormalProofTheory L Gamma}
+        {mpGamma: MinimunPropositionalLogic L Gamma}
+        {ipGamma: IntuitionisticPropositionalLogic L Gamma}.
+
+Definition DDC: context -> Prop := fun Psi =>
+  derivable_closed Psi /\ orp_witnessed Psi /\ consistent Psi.
+
+Lemma DER: at_least_derivable_closed DDC.
+Proof. hnf; intros ? [? [? ?]]; auto. Qed.
+
+Lemma ORP: at_least_orp_witnessed DDC.
+Proof. hnf; intros ? [? [? ?]]; auto. Qed.
+
+Lemma CONSI: at_least_consistent DDC.
+Proof. hnf; intros ? [? [? ?]]; auto. Qed.
+
+Lemma LIN_DER: Linderbaum_derivable DDC.
+Proof.
+  hnf; intros.
+  pose proof Lindenbaum_lemma
+    (PropositionalLanguage.formula_countable Var CV)  _ _ H
+  as [Psi [? [? ?]]].
+  exists (exist _ Psi H2); auto.
+Qed.
+
+Definition canonical_frame: KripkeSemantics.frame :=
+  KripkeSemantics.Build_frame (sig DDC) (fun a b => Included _ (proj1_sig a) (proj1_sig b)).
+
+Definition canonical_eval: Var -> KripkeSemantics.sem canonical_frame :=
+  fun p a => proj1_sig a (PropositionalLanguage.varp p).
+
+Definition canonical_Kmodel: @Kmodel (KripkeSemantics.MD Var) (KripkeSemantics.kMD Var) :=
+  KripkeSemantics.Build_Kmodel Var canonical_frame canonical_eval.
+
+Definition rel: bijection (Kworlds canonical_Kmodel) (sig DDC) := bijection_refl.
+
+Definition H_R:
+  forall m n Phi Psi, rel m Phi -> rel n Psi ->
+    (m <= n <-> Included _ (proj1_sig Phi) (proj1_sig Psi)).
+Proof.
+  intros.
+  change (m = Phi) in H.
+  change (n = Psi) in H0.
+  subst; reflexivity.
+Qed.
+
+Lemma TRUTH:
+  forall x: expr, forall m Phi, rel m Phi ->
+    (KRIPKE: canonical_Kmodel, m |= x <-> proj1_sig Phi x).
+Proof.
+  induction x.
+  + exact (truth_lemma_andp DDC rel DER x1 x2 IHx1 IHx2).
+  + exact (truth_lemma_orp DDC rel DER ORP x1 x2 IHx1 IHx2).
+  + exact (truth_lemma_impp DDC rel H_R DER LIN_DER x1 x2 IHx1 IHx2).
+  + exact (truth_lemma_falsep DDC rel CONSI).
+  + intros; change (m = Phi) in H; subst; reflexivity.
+Qed.
+
+End General_Completeness.
+
+Section Intuitionistic_Completeness.
+
+Instance Intuitionistic_nG: NormalProofTheory L Intuitionistic_G := IntuitionisticLogic.nG Var.
+Instance Intuitionistic_mpG: MinimunPropositionalLogic L Intuitionistic_G := IntuitionisticLogic.mpG Var.
+Instance Intuitionistic_ipG: IntuitionisticPropositionalLogic L Intuitionistic_G := IntuitionisticLogic.ipG Var.
+
+Import Logic.PropositionalLogic.DeepEmbedded.KripkeSemantics.
+
+Theorem complete_intuitionistic_Kripke_all:
+  strongly_complete Intuitionistic_G Kripke_SM
+    (KripkeModelClass _ (Kmodel_Monotonic + Kmodel_PreOrder)).
+Proof.
+  apply (@general_completeness _ _ _ _ _ _ _ _ _ _ DDC rel LIN_DER DER TRUTH).
+  constructor; hnf.
+  + intros.
+    exact (denote_monotonic DDC rel H_R
+             (PropositionalLanguage.varp v)
+             (TRUTH (PropositionalLanguage.varp v))).
+  + exact (po_R DDC rel H_R).
+Qed.
+
+End Intuitionistic_Completeness.
+  
+Section DeMorgan_Completeness.
+
+Instance DeMorgan_nG: NormalProofTheory L DeMorgan_G := DeMorganLogic.nG Var.
+Instance DeMorgan_mpG: MinimunPropositionalLogic L DeMorgan_G := DeMorganLogic.mpG Var.
+Instance DeMorgan_ipG: IntuitionisticPropositionalLogic L DeMorgan_G := DeMorganLogic.ipG Var.
+Instance DeMorgan_dmpG: DeMorganPropositionalLogic L DeMorgan_G := DeMorganLogic.dmpG Var.
+
+Import Logic.PropositionalLogic.DeepEmbedded.KripkeSemantics.
+
+Theorem complete_DeMorgan_Kripke_branch_join:
+  strongly_complete DeMorgan_G Kripke_SM
+    (KripkeModelClass _ (Kmodel_Monotonic + Kmodel_PreOrder + Kmodel_BranchJoin)).
+Proof.
+  apply (@general_completeness _ _ _ _ _ _ _ _ _ _ DDC rel LIN_DER DER TRUTH).
+  constructor; [split |]; hnf.
+  + intros.
+    exact (denote_monotonic DDC rel H_R
+             (PropositionalLanguage.varp v)
+             (TRUTH (PropositionalLanguage.varp v))).
+  + exact (po_R DDC rel H_R).
+  + exact (DeMorgan_canonical_branch_join DDC rel H_R DER ORP CONSI LIN_DER).
+Qed.
+
+End DeMorgan_Completeness.
+
+Section GodelDummett_Completeness.
+
+Instance GodelDummett_nG: NormalProofTheory L GodelDummett_G := GodelDummettLogic.nG Var.
+Instance GodelDummett_mpG: MinimunPropositionalLogic L GodelDummett_G := GodelDummettLogic.mpG Var.
+Instance GodelDummett_ipG: IntuitionisticPropositionalLogic L GodelDummett_G := GodelDummettLogic.ipG Var.
+Instance GodelDummett_gdpG: GodelDummettPropositionalLogic L GodelDummett_G := GodelDummettLogic.gdpG Var.
+
+Import Logic.PropositionalLogic.DeepEmbedded.KripkeSemantics.
+
+Theorem complete_GodelDummett_Kripke_no_branch:
+  strongly_complete GodelDummett_G Kripke_SM
+    (KripkeModelClass _ (Kmodel_Monotonic + Kmodel_PreOrder + Kmodel_NoBranch)).
+Proof.
+  apply (@general_completeness _ _ _ _ _ _ _ _ _ _ DDC rel LIN_DER DER TRUTH).
+  constructor; [split |]; hnf.
+  + intros.
+    exact (denote_monotonic DDC rel H_R
+             (PropositionalLanguage.varp v)
+             (TRUTH (PropositionalLanguage.varp v))).
+  + exact (po_R DDC rel H_R).
+  + exact (GodelDummett_canonical_no_branch DDC rel H_R DER ORP).
+Qed.
+
+End GodelDummett_Completeness.
+
+Section Classical_Completeness.
+
+Instance Classical_nG: NormalProofTheory L Classical_G := ClassicalLogic.nG Var.
+Instance Classical_mpG: MinimunPropositionalLogic L Classical_G := ClassicalLogic.mpG Var.
+Instance Classical_ipG: IntuitionisticPropositionalLogic L Classical_G := ClassicalLogic.ipG Var.
+Instance Classical_cpG: ClassicalPropositionalLogic L Classical_G := ClassicalLogic.cpG Var.
+
+Import Logic.PropositionalLogic.DeepEmbedded.KripkeSemantics.
+
+Theorem complete_Classical_Kripke_identity:
+  strongly_complete Classical_G Kripke_SM
+    (KripkeModelClass _ (Kmodel_Monotonic + Kmodel_PreOrder + Kmodel_Identity)).
+Proof.
+  apply (@general_completeness _ _ _ _ _ _ _ _ _ _ DDC rel LIN_DER DER TRUTH).
+  constructor; [split |]; hnf.
+  + intros.
+    exact (denote_monotonic DDC rel H_R
+             (PropositionalLanguage.varp v)
+             (TRUTH (PropositionalLanguage.varp v))).
+  + exact (po_R DDC rel H_R).
+  + exact (classical_canonical_ident DDC rel H_R DER ORP CONSI).
+Qed.
+
+End Classical_Completeness.
+
+End Complete.
